p4cub: more file reorganization

deps/poulet4/lib/P4cub/SmallStep/SSSemantics.v
@@ -1,270 +1,11 @@
+Set Warnings "-custom-entry-overridden".
 Require Export Poulet4.P4cub.Static.Check.
-Require Import Coq.Bool.Bool Coq.ZArith.BinIntDef
-        Coq.ZArith.BinInt Coq.Arith.Compare_dec Coq.micromega.Lia
-        Poulet4.P4cub.Syntax.SynEquiv
-        Poulet4.P4cub.Syntax.SynAuxilary
-        Poulet4.P4cub.Syntax.SynIndPrincip.
-        (*Poulet4.P4cub.Static.StaticIndPrincip.*)
+Require Import Poulet4.P4cub.SmallStep.SSValue
+        Poulet4.P4cub.SmallStep.SSUtil
+        Coq.ZArith.BinInt.
 
 (** Notation entries. *)
 Declare Custom Entry p4kstmt.
-
-(** * Small-Step Values *)
-Module IsValue.
-  Module P := P4cub.
-  Module E := P.Expr.
-  Module F := P.F.
-
-  Import P.P4cubNotations.
-
-  Inductive value {tags_t : Type} : E.e tags_t -> Prop :=
-  | value_bool (b : bool) (i : tags_t) :
-      value <{ BOOL b @ i }>
-  | value_bit (w : positive) (n : Z) (i : tags_t) :
-      value <{ w W n @ i }>
-  | value_int (w : positive) (z : Z) (i : tags_t) :
-      value <{ w S z @ i }>
-  | value_tuple (es : list (E.e tags_t)) (i : tags_t) :
-      Forall value es ->
-      value <{ tup es @ i }>
-  | value_struct (fs : F.fs string (E.t * E.e tags_t))
-                 (i : tags_t) :
-      F.predfs_data (value ∘ snd) fs ->
-      value <{ struct { fs } @ i }>
-  | value_header (fs : F.fs string (E.t * E.e tags_t))
-                 (b : E.e tags_t) (i : tags_t) :
-      value b ->
-      F.predfs_data (value ∘ snd) fs ->
-      value <{ hdr { fs } valid:=b @ i }>
-  | value_error (err : option (string)) (i : tags_t) :
-      value <{ Error err @ i }>
-  | value_matchkind (mk : E.matchkind) (i : tags_t) :
-      value <{ Matchkind mk @ i }>
-  | value_headerstack (fs : F.fs string (E.t))
-                      (hs : list (E.e tags_t)) (n : positive)
-                      (ni : Z) (i : tags_t) :
-      Forall value hs ->
-      value <{ Stack hs:fs[n] nextIndex:=ni @ i }>.
-  (**[]*)
-
-  Section IsValueInduction.
-    Variable tags_t : Type.
-
-    Variable P : E.e tags_t -> Prop.
-
-    Hypothesis HBool : forall b i, P <{ BOOL b @ i }>.
-
-    Hypothesis HBit : forall w n i, P <{ w W n @ i }>.
-
-    Hypothesis HInt : forall w z i, P <{ w S z @ i }>.
-
-    Hypothesis HTuple : forall es i,
-      Forall value es ->
-      Forall P es ->
-      P <{ tup es @ i }>.
-
-    Hypothesis HStruct : forall fs i,
-        F.predfs_data (value ∘ snd) fs ->
-        F.predfs_data (P ∘ snd) fs ->
-        P <{ struct { fs } @ i }>.
-
-    Hypothesis HHeader : forall fs b i,
-        value b ->
-        P b ->
-        F.predfs_data (value ∘ snd) fs ->
-        F.predfs_data (P ∘ snd) fs ->
-        P <{ hdr { fs } valid:=b @ i }>.
-
-    Hypothesis HError : forall err i, P <{ Error err @ i }>.
-
-    Hypothesis HMatchkind : forall mk i, P <{ Matchkind mk @ i }>.
-
-    Hypothesis HStack : forall fs hs n ni i,
-        Forall value hs ->
-        Forall P hs ->
-        P <{ Stack hs:fs[n] nextIndex:=ni @ i }>.
-
-    Definition custom_value_ind : forall (e : E.e tags_t),
-        value e -> P e :=
-      fix vind (e : E.e tags_t) (H : value e) : P e :=
-        let fix lind {es : list (E.e tags_t)}
-                (Hes : Forall value es) : Forall P es :=
-            match Hes with
-            | Forall_nil _ => Forall_nil _
-            | Forall_cons _ Hh Ht => Forall_cons _ (vind _ Hh) (lind Ht)
-            end in
-        let fix find {A : Type} {fs : F.fs string (A * E.e tags_t)}
-                (Hfs : F.predfs_data (value ∘ snd) fs) :
-              F.predfs_data (P ∘ snd) fs :=
-            match Hfs with
-            | Forall_nil _ => Forall_nil _
-            | Forall_cons _ Hh Ht => Forall_cons _ (vind _ Hh) (find Ht)
-            end in
-        match H with
-        | value_bool b i => HBool b i
-        | value_bit w n i => HBit w n i
-        | value_int w z i => HInt w z i
-        | value_tuple _ i Hes => HTuple _ i Hes (lind Hes)
-        | value_struct _ i Hfs => HStruct _ i Hfs (find Hfs)
-        | value_header _ _ i Hb Hfs
-          => HHeader _ _ i Hb (vind _ Hb) Hfs (find Hfs)
-        | value_error err i => HError err i
-        | value_matchkind mk i => HMatchkind mk i
-        | value_headerstack fs _ n ni i Hhs => HStack fs _ n ni i Hhs (lind Hhs)
-        end.
-  End IsValueInduction.
-
-  Section Lemmas.
-    Import F.FieldTactics.
-
-    Hint Constructors value : core.
-    Hint Extern 0 => inv_Forall_cons : core.
-
-    Lemma value_exm : forall {tags_t : Type} (e : E.e tags_t), value e \/ ~ value e.
-    Proof.
-      induction e using custom_e_ind; auto 2;
-      try (right; intros H'; inv H'; contradiction).
-      - assert (Forall value es \/ ~ Forall value es).
-        { ind_list_Forall; intuition. }
-        intuition. right; intros H'; inv H'. contradiction.
-      - assert (F.predfs_data (value ∘ snd) fields \/
-                ~ F.predfs_data (value ∘ snd) fields).
-        { ind_list_predfs; unfold F.predfs_data in *; intuition. }
-        intuition. right; intros H'; inv H'. contradiction.
-      - assert (F.predfs_data (value ∘ snd) fields \/
-                ~ F.predfs_data (value ∘ snd) fields).
-        { ind_list_predfs; unfold F.predfs_data in *; intuition. }
-        intuition; right; intros H'; inv H'; contradiction.
-      - assert (Forall value hs \/ ~ Forall value hs).
-        { ind_list_Forall; intuition. }
-        intuition. right; intros H'; inv H'. contradiction.
-    Qed.
-  End Lemmas.
-
-  Inductive lvalue {tags_t : Type} : E.e tags_t -> Prop :=
-  | lvalue_var x τ i :
-      lvalue <{ Var x:τ @ i }>
-  | lvalue_member lv τ x i :
-      lvalue lv ->
-      lvalue <{ Mem lv:τ dot x @ i }>
-  | lvalue_access lv idx i :
-      lvalue lv ->
-      lvalue <{ Access lv[idx] @ i }>.
-  (**[]*)
-
-  Module CanonicalForms.
-    Ltac invert_value :=
-      match goal with
-      | H: value _ |- _ => inv H
-      end.
-    (**[]*)
-
-    Ltac invert_expr_check :=
-      match goal with
-      | H: ⟦ _, _ ⟧ ⊢ _ ∈ _ |- _ => inv H
-      end.
-    (**[]*)
-
-    Ltac invert_canonical := invert_value; invert_expr_check.
-
-    Ltac crush_canonical := intros; invert_canonical; eauto 4.
-
-    Section CanonicalForms.
-      Variable errs : errors.
-
-      Variable Γ : gamma.
-
-      Context {tags_t : Type}.
-
-      Variable v : E.e tags_t.
-
-      Hypothesis Hv : value v.
-
-      Lemma canonical_forms_bool :
-        ⟦ errs, Γ ⟧ ⊢ v ∈ Bool -> exists b i, v = <{ BOOL b @ i }>.
-      Proof. crush_canonical. Qed.
-
-      Lemma canonical_forms_bit : forall w,
-          ⟦ errs, Γ ⟧ ⊢ v ∈ bit<w> -> exists n i, v = <{ w W n @ i }>.
-      Proof. crush_canonical. Qed.
-
-      Lemma canonical_forms_int : forall w,
-          ⟦ errs, Γ ⟧ ⊢ v ∈ int<w> -> exists z i, v = <{ w S z @ i }>.
-      Proof. crush_canonical. Qed.
-
-      Lemma canonical_forms_tuple : forall ts,
-          ⟦ errs, Γ ⟧ ⊢ v ∈ tuple ts -> exists es i, v = <{ tup es @ i }>.
-      Proof. crush_canonical. Qed.
-
-      Lemma canonical_forms_struct : forall ts,
-          ⟦ errs, Γ ⟧ ⊢ v ∈ struct { ts } -> exists fs i, v = <{ struct { fs } @ i }>.
-      Proof. crush_canonical. Qed.
-
-      Lemma canonical_forms_header : forall ts,
-          ⟦ errs, Γ ⟧ ⊢ v ∈ hdr { ts } -> exists fs b i, v = <{ hdr { fs } valid:=b @ i }>.
-      Proof. crush_canonical. Qed.
-
-      Lemma canonical_forms_error :
-        ⟦ errs, Γ ⟧ ⊢ v ∈ error -> exists err i, v = <{ Error err @ i }>.
-      Proof. crush_canonical. Qed.
-
-      Lemma canonical_forms_matchkind :
-        ⟦ errs, Γ ⟧ ⊢ v ∈ matchkind -> exists mk i, v = <{ Matchkind mk @ i }>.
-      Proof. crush_canonical. Qed.
-
-      Lemma canonical_forms_headerstack : forall ts n,
-          ⟦ errs, Γ ⟧ ⊢ v ∈ stack ts[n] ->
-          exists hs ni i, v = <{ Stack hs:ts[n] nextIndex:= ni @ i }>.
-      Proof. crush_canonical. Qed.
-    End CanonicalForms.
-
-    Ltac inv_eq_val_expr :=
-      match goal with
-      | H: <{ BOOL _ @ _ }> = <{ BOOL _ @ _ }> |- _ => inv H
-      | H: <{ _ W _ @ _ }> = <{ _ W _ @ _ }> |- _ => inv H
-      | H: <{ _ S _ @ _ }> = <{ _ S _ @ _ }> |- _ => inv H
-      | H: <{ tup _ @ _ }> = <{ tup _ @ _ }> |- _ => inv H
-      | H: <{ struct { _ } @ _ }> = <{ struct { _ } @ _ }> |- _ => inv H
-      | H: <{ hdr { _ } valid:=_ @ _ }> = <{ hdr { _ } valid:=_ @ _ }>
-        |- _ => inv H
-      | H: <{ Stack _:_[_] nextIndex:=_ @ _ }> = <{ Stack _:_[_] nextIndex:=_ @ _ }>
-        |- _ => inv H
-      end.
-    (**[]*)
-
-    Ltac assert_canonical_forms :=
-      match goal with
-      | Hv: value ?v, Ht: ⟦ _, _ ⟧ ⊢ ?v ∈ Bool |- _
-        => pose proof canonical_forms_bool _ _ _ Hv Ht as [? [? Hcanon]];
-          inv Hcanon; inv Hv; inv Ht
-      | Hv: value ?v, Ht: ⟦ _, _ ⟧ ⊢ ?v ∈ bit<_> |- _
-        => pose proof canonical_forms_bit _ _ _ Hv _ Ht as [? [? Hcanon]];
-          inv Hcanon; inv Hv; inv Ht
-      | Hv: value ?v, Ht: ⟦ _, _ ⟧ ⊢ ?v ∈ int<_> |- _
-        => pose proof canonical_forms_int _ _ _ Hv _ Ht as [? [? Hcanon]];
-          inv Hcanon; inv Hv; inv Ht
-      | Hv: value ?v, Ht: ⟦ _, _ ⟧ ⊢ ?v ∈ tuple _ |- _
-        => pose proof canonical_forms_tuple _ _ _ Hv _ Ht as [? [? Hcanon]];
-          inv Hcanon; inv Hv; inv Ht
-      | Hv: value ?v, Ht: ⟦ _, _ ⟧ ⊢ ?v ∈ struct { _ } |- _
-        => pose proof canonical_forms_struct _ _ _ Hv _ Ht as [? [? Hcanon]];
-          inv Hcanon; inv Hv; inv Ht
-      | Hv: value ?v, Ht: ⟦ _, _ ⟧ ⊢ ?v ∈ hdr { _ } |- _
-        => pose proof canonical_forms_header _ _ _ Hv _ Ht as [? [? [? Hcanon]]];
-          inv Hcanon; inv Hv; inv Ht
-      | Hv: value ?v, Ht: ⟦ _, _ ⟧ ⊢ ?v ∈ error |- _
-        => pose proof canonical_forms_error _ _ _ Hv Ht as [? [? Hcanon]];
-          inv Hcanon; inv Hv; inv Ht
-      | Hv: value ?v, Ht: ⟦ _, _ ⟧ ⊢ ?v ∈ matchkind |- _
-        => pose proof canonical_forms_matchkind _ _ _ Hv Ht as [? [? Hcanon]];
-          inv Hcanon; inv Hv; inv Ht
-      | Hv: value ?v, Ht: ⟦ _, _ ⟧ ⊢ ?v ∈ stack _[_] |- _
-        => pose proof canonical_forms_headerstack _ _ _ Hv _ _ Ht as [? [? [? Hcanon]]];
-          inv Hcanon; inv Hv; inv Ht
-      end.
-    (**[]*)
-  End CanonicalForms.
-End IsValue.
 
 Module Step.
   Module P := P4cub.
@@ -274,637 +15,20 @@ Module Step.
   Module PT := ProperType.
   Module PR := P.Parser.
   Import P.P4cubNotations Env.EnvNotations.
-  Module V := IsValue.
 
-  Section StepDefs.
-    Import TypeEquivalence ProperType
-           F.FieldTactics P4ArithTactics.
-
-    Context {tags_t : Type}.
-
-    (** Expression environment. *)
-    Definition eenv : Type := Env.t (string) (E.e tags_t).
-
-    (** Bit-slicing. *)
-    Definition eval_slice (hi lo : positive) (v : E.e tags_t) : option (E.e tags_t) :=
-      match v with
-      | <{ _ W z @ i }>
-      | <{ _ S z @ i }>
-        => let w' := (hi - lo + 1)%positive in
-        Some $ E.EBit w'
-             (BitArith.mod_bound w' $
-              BitArith.bitstring_slice z hi lo) i
-      | _ => None
-      end.
-    (**[]*)
-
-    Definition eval_cast
-               (target : E.t) (v : E.e tags_t) : option (E.e tags_t) :=
-      match target, v with
-      | {{ bit<xH> }}, <{ TRUE @ i }>         => Some (E.EBit 1%positive 1%N i)
-      | {{ bit<xH> }}, <{ FALSE @ i }>        => Some (E.EBit 1%positive 0%N i)
-      | {{ Bool }}, E.EBit 1%positive 1%N i => Some <{ TRUE @ i }>
-      | {{ Bool }}, E.EBit 1%positive 0%N i => Some <{ FALSE @ i }>
-      | {{ bit<w> }}, E.EInt _ z i
-        => let n := BitArith.mod_bound w z in
-          Some <{ w W n @ i }>
-      | {{ int<w> }}, <{ _ W n @ i }>
-        => let z := IntArith.mod_bound w n in
-          Some <{ w S z @ i }>
-      | {{ bit<w> }}, <{ _ W n @ i }>
-        => let n := BitArith.mod_bound w n in
-          Some <{ w W n @ i }>
-      | {{ int<w> }}, <{ _ S z @ i}>
-        => let z := IntArith.mod_bound w z in
-          Some <{ w S z @ i }>
-      | {{ struct { fs } }}, <{ tup vs @ i }>
-        => Some $ E.EStruct (combine (F.keys fs) $ combine (F.values fs) vs) i
-      | {{ hdr { fs } }}, <{ tup vs @ i }>
-        => Some
-            $ E.EHeader
-            (combine (F.keys fs) $ combine (F.values fs) vs) <{ TRUE @ i }> i
-      | _, _ => None
-      end.
-    (**[]*)
-
-    (** Default (value) Expression. *)
-    Fixpoint edefault (i : tags_t) (τ : E.t) : E.e tags_t :=
-      let fix lstruct (ts : list (E.t)) : list (E.e tags_t) :=
-          match ts with
-          | []     => []
-          | τ :: ts => edefault i τ :: lstruct ts
-          end in
-      let fix fstruct (fs : F.fs string (E.t))
-          : F.fs string (E.t * E.e tags_t) :=
-          match fs with
-          | [] => []
-          | (x, τ) :: fs => (x, (τ, edefault i τ)) :: fstruct fs
-          end in
-      match τ with
-      | {{ Bool }} => <{ BOOL false @ i }>
-      | {{ bit<w> }} => E.EBit w 0%Z i
-      | {{ int<w> }} => E.EInt w 0%Z i
-      | {{ error }} => <{ Error None @ i }>
-      | {{ matchkind }} => <{ Matchkind exact @ i }>
-      | {{ tuple ts }} => E.ETuple (lstruct ts) i
-      | {{ struct { fs } }} => E.EStruct (fstruct fs) i
-      | {{ hdr { fs } }} => E.EHeader (fstruct fs) <{ BOOL false @ i }> i
-      | {{ stack tfs[n] }}
-          => let tefs := fstruct tfs in
-            let hs :=
-                repeat
-                <{ hdr { tefs } valid:= BOOL false @ i @ i }>
-                (Pos.to_nat n) in
-            E.EHeaderStack tfs hs n 0%Z i
-      end.
-    (**[]*)
-
-    (** Unary Operations. *)
-    Definition eval_uop (op : E.uop) (e : E.e tags_t) : option (E.e tags_t) :=
-      match op, e with
-      | _{ ! }_, <{ BOOL b @ i }>
-        => let b' := negb b in Some <{ BOOL b' @ i }>
-      | _{ ~ }_, <{ w W n @ i }>
-        => let n' := BitArith.bit_not w n in Some <{ w W n' @ i }>
-      | _{ ~ }_, <{ w S n @ i }>
-        => let n' := IntArith.bit_not w n in Some <{ w S n' @ i }>
-      | _{ - }_, <{ w W z @ i }>
-        => let z' := BitArith.neg w z in Some <{ w W z' @ i }>
-      | _{ - }_, <{ w S z @ i }>
-        => let z' := IntArith.neg w z in Some <{ w S z' @ i }>
-      | _{ isValid }_, <{ hdr { _ } valid:=b @ i }> => Some b
-      | _{ setValid }_, <{ hdr { fs } valid:=_ @ i }>
-        => Some <{ hdr { fs } valid:=TRUE @ i @ i}>
-      | _{ setInValid }_, <{ hdr { fs } valid:=b @ i }>
-        => Some <{ hdr { fs } valid:=FALSE @ i @ i }>
-      | _{ Size }_, <{ Stack _:_[size] nextIndex:=_ @ i }>
-        => let w := 32%positive in
-          let s := Zpos size in Some <{ w W s @ i }>
-      | _{ Next }_, <{ Stack hs:_[_] nextIndex:=ni @ _ }>
-        => nth_error hs $ Z.to_nat ni
-      | _{ Push p }_, <{ Stack hs:ts[n] nextIndex:=ni @ i }>
-        => let pnat := Pos.to_nat p in
-          let sizenat := Pos.to_nat n in
-          let hdefault :=
-              E.EHeader
-                (F.map (fun τ => (τ, edefault i τ)) ts)
-              <{ BOOL false @ i }> i in
-          if lt_dec pnat sizenat then
-            let new_hdrs := repeat hdefault pnat in
-            let remains := firstn (sizenat - pnat) hs in
-            Some $ E.EHeaderStack ts (new_hdrs ++ remains) n
-                 (Z.min (ni + Zpos p)%Z (Z.pos n - 1)%Z) i
-          else
-            let new_hdrs := repeat hdefault sizenat in
-            Some $ E.EHeaderStack ts new_hdrs n (Z.pos n - 1)%Z i
-      | _{ Pop p }_, <{ Stack hs:ts[n] nextIndex:=ni @ i }>
-        => let pnat := Pos.to_nat p in
-          let sizenat := Pos.to_nat n in
-          let hdefault :=
-              E.EHeader
-                (F.map (fun τ => (τ, edefault i τ)) ts)
-              <{ BOOL false @ i }> i in
-          if lt_dec pnat sizenat then
-            let new_hdrs := repeat hdefault pnat in
-            let remains := skipn pnat hs in
-            Some $ E.EHeaderStack ts (remains ++ new_hdrs) n
-                 (Z.max 0 (ni - Zpos p)%Z) i
-          else
-            let new_hdrs := repeat hdefault sizenat in
-            Some $ E.EHeaderStack ts new_hdrs n 0%N i
-      | _, _ => None
-      end.
-    (**[]*)
-
-    (** Binary operations. *)
-    Definition eval_bop
-               (op : E.bop) (v1 v2 : E.e tags_t) (i : tags_t) : option (E.e tags_t) :=
-      match op, v1, v2 with
-      | +{ + }+, <{ w W n1 @ _ }>, <{ _ W n2 @ _ }>
-        => Some $ E.EBit w (BitArith.plus_mod w n1 n2) i
-      | +{ + }+, <{ w S z1 @ _ }>, <{ _ S z2 @ _ }>
-        => Some $ E.EInt w (IntArith.plus_mod w z1 z2) i
-      | +{ |+| }+, <{ w W n1 @ _ }>, <{ _ W n2 @ _ }>
-        => Some $ E.EBit w (BitArith.plus_sat w n1 n2) i
-      | +{ |+| }+,  <{ w S z1 @ _ }>, <{ _ S z2 @ _ }>
-        => Some $ E.EInt w (IntArith.plus_sat w z1 z2) i
-      | +{ - }+, <{ w W n1 @ _ }>, <{ _ W n2 @ _ }>
-        => Some $ E.EBit w (BitArith.minus_mod w n1 n2) i
-      | +{ - }+, <{ w S z1 @ _ }>, <{ _ S z2 @ _ }>
-        => Some $ E.EInt w (IntArith.minus_mod w z1 z2) i
-      | +{ |-| }+, <{ w W n1 @ _ }>, <{ _ W n2 @ _ }>
-        => Some $ E.EBit w (BitArith.minus_sat w n1 n2) i
-      | +{ |-| }+, <{ w S z1 @ _ }>, <{ _ S z2 @ _ }>
-        => Some $ E.EInt w (IntArith.minus_sat w z1 z2) i
-      | +{ × }+, <{ w W n1 @ _ }>, <{ _ W n2 @ _ }>
-        => Some $ E.EBit w (BitArith.mult_mod w n1 n2) i
-      | +{ × }+, <{ w S n1 @ _ }>, <{ _ S n2 @ _ }>
-        => Some $ E.EInt w (IntArith.mult_mod w n1 n2) i
-      | +{ << }+, <{ w W n1 @ _ }>, <{ _ W n2 @ _ }>
-        => Some $ E.EBit w (BitArith.shift_left w n1 n2) i
-      | +{ << }+, <{ w S z1 @ _ }>, <{ _ W z2 @ _ }>
-        => Some $ E.EInt w (IntArith.shift_left w z1 z2) i
-      | +{ >> }+, <{ w W n1 @ _ }>, <{ _ W n2 @ _ }>
-        => Some $ E.EBit w (BitArith.shift_right w n1 n2) i
-      | +{ >> }+, <{ w S z1 @ _ }>, <{ _ W z2 @ _ }>
-        => Some $ E.EInt w (IntArith.shift_right w z1 z2) i
-      | +{ & }+, <{ w W n1 @ _ }>, <{ _ W n2 @ _ }>
-        => Some $ E.EBit w (BitArith.bit_and w n1 n2) i
-      | +{ & }+, <{ w S z1 @ _ }>, <{ _ S z2 @ _ }>
-        => Some $ E.EInt w (IntArith.bit_and w z1 z2) i
-      | +{ ^ }+, <{ w W n1 @ _ }>, <{ _ W n2 @ _ }>
-        => Some $ E.EBit w (BitArith.bit_xor w n1 n2) i
-      | +{ ^ }+, <{ w S z1 @ _ }>, <{ _ S z2 @ _ }>
-        => Some $ E.EInt w (IntArith.bit_xor w z1 z2) i
-      | +{ | }+, <{ w W n1 @ _ }>, <{ _ W n2 @ _ }>
-        => Some $ E.EBit w (BitArith.bit_or w n1 n2) i
-      | +{ | }+, <{ w S z1 @ _ }>, <{ _ S z2 @ _ }>
-        => Some $ E.EInt w (IntArith.bit_or w z1 z2) i
-      | +{ <= }+, <{ w W n1 @ _ }>, <{ _ W n2 @ _ }> => Some $ E.EBool (n1 <=? n2)%Z i
-      | +{ <= }+, <{ w S z1 @ _ }>, <{ _ S z2 @ _ }> => Some $ E.EBool (z1 <=? z2)%Z i
-      | +{ < }+, <{ w W n1 @ _ }>, <{ _ W n2 @ _ }> => Some $ E.EBool (n1 <? n2)%Z i
-      | +{ < }+, <{ w S z1 @ _ }>, <{ _ S z2 @ _ }> => Some $ E.EBool (z1 <? z2)%Z i
-      | +{ >= }+, <{ w W n1 @ _ }>, <{ _ W n2 @ _ }> => Some $ E.EBool (n2 <=? n1)%Z i
-      | +{ >= }+, <{ w S z1 @ _ }>, <{ _ S z2 @ _ }> => Some $ E.EBool (z2 <=? z1)%Z i
-      | +{ > }+, <{ w W n1 @ _ }>, <{ _ W n2 @ _ }> => Some $ E.EBool (n2 <? n1)%Z i
-      | +{ > }+, <{ w S z1 @ _ }>, <{ _ S z2 @ _ }> => Some $ E.EBool (z2 <? z1)%Z i
-      | +{ && }+, <{ BOOL b1 @ _ }>, <{ BOOL b2 @ _ }> => Some $ E.EBool (b1 && b2) i
-      | +{ || }+, <{ BOOL b1 @ _ }>, <{ BOOL b2 @ _ }> => Some $ E.EBool (b1 || b2) i
-      | +{ == }+, _, _ => Some $ E.EBool (ExprEquivalence.eqbe v1 v2) i
-      | +{ != }+, _, _ => Some $ E.EBool (negb $ ExprEquivalence.eqbe v1 v2) i
-      | +{ ++ }+, <{ w1 W n1 @ _ }>, <{ w2 W n2 @ _ }>
-      | +{ ++ }+, <{ w1 W n1 @ _ }>, <{ w2 S n2 @ _ }>
-        => Some $ E.EBit (w1 + w2)%positive (BitArith.concat w1 w2 n1 n2) i
-      | +{ ++ }+, <{ w1 S n1 @ _ }>, <{ w2 S n2 @ _ }>
-      | +{ ++ }+, <{ w1 S n1 @ _ }>, <{ w2 W n2 @ _ }>
-        => Some $ E.EInt (w1 + w2)%positive (IntArith.concat w1 w2 n1 n2) i
-      | _, _, _ => None
-      end.
-    (**[]*)
-
-    (** Get header stack data from value. *)
-    Definition header_stack_data (v : E.e tags_t)
-      : option (positive * Z *
-                F.fs string (E.t) *
-                (list (E.e tags_t))) :=
-      match v with
-      | <{ Stack hs:ts[n] nextIndex:=ni @ _}> => Some (n,ni,ts,hs)
-      | _ => None
-      end.
-    (**[]*)
-
-    Definition eval_member (x : string) (v : E.e tags_t) : option (E.e tags_t) :=
-      match v with
-      | <{ struct { vs } @ _ }>
-      | <{ hdr { vs } valid:=_ @ _ }> => vs ▷ F.get x >>| snd
-      | _                             => None
-      end.
-    (**[]*)
-
-    Section Edefault.
-      Local Hint Constructors V.value : core.
-
-      Lemma value_edefault : forall i τ, V.value (edefault i τ).
-      Proof.
-        induction τ using custom_t_ind; unravel; auto 1;
-        try (constructor; apply repeat_Forall); constructor; auto 1;
-        try (ind_list_predfs; unfold F.predfs_data in * );
-        try ind_list_Forall; unravel in *; auto 4.
-      Qed.
-    End Edefault.
-
-    Section HelpersType.
-      Local Hint Constructors check_expr : core.
-      Local Hint Extern 0 => bit_bounded : core.
-      Local Hint Extern 0 => int_bounded : core.
-
-      Import V.CanonicalForms.
-
-      Lemma eval_slice_types : forall errs Γ v v' τ hi lo w,
-          eval_slice hi lo v = Some v' ->
-          V.value v ->
-          (lo <= hi < w)%positive ->
-          numeric_width w τ ->
-          ⟦ errs, Γ ⟧ ⊢ v ∈ τ ->
-          let w' := (hi - lo + 1)%positive in
-          ⟦ errs, Γ ⟧ ⊢ v' ∈ bit<w'>.
-      Proof.
-        intros errs Γ v v' τ hi lo w Heval Hv Hw Hnum Ht w'; subst w';
-        inv Hnum; assert_canonical_forms; unravel in *; inv Heval; auto 2.
-      Qed.
-
-      Local Hint Resolve BitArith.bound0 : core.
-      Local Hint Resolve BitArith.bound1 : core.
-      Local Hint Resolve IntArith.bound0 : core.
-
-      Lemma eval_cast_types : forall errs Γ τ τ' v v',
-          eval_cast τ' v = Some v' ->
-          V.value v ->
-          proper_cast τ τ' ->
-          ⟦ errs, Γ ⟧ ⊢ v ∈ τ ->
-          ⟦ errs, Γ ⟧ ⊢ v' ∈ τ'.
-      Proof.
-        intros errs Γ τ τ' v v' Heval Hv Hpc Ht;
-        inv Hpc; assert_canonical_forms; unravel in *;
-        try match goal with
-            | H: context [ if ?b then _ else _ ]
-              |- _ => destruct b eqn:?
-            end; try (inv Heval; auto 2; assumption).
-        - destruct x; try (inv Heval; auto 2; assumption).
-          destruct p; inv Heval; auto 2.
-        - destruct w; inv Heval; auto 2.
-        - destruct w2; inv Heval; auto 2.
-        - inv Heval. constructor.
-          generalize dependent fs.
-          ind_list_Forall; intros [| [? ?] ?] ?;
-          unravel in *; try inv_Forall2_cons;
-          constructor; try split;
-          unravel; try apply IHx; auto 2.
-        - inv Heval; constructor; auto 1.
-          + apply pn_header. rewrite F.predfs_data_map. assumption.
-          + clear x0 H0. generalize dependent fs.
-            ind_list_Forall; intros [| [? ?] ?] ? ;
-            unravel in *; try inv_Forall2_cons;
-            constructor; try split;
-            unravel; try apply IHx; auto 2.
-      Qed.
-
-      Lemma eval_bop_types : forall Γ errs op τ1 τ2 τ (i : tags_t) v1 v2 v,
-          bop_type op τ1 τ2 τ ->
-          V.value v1 -> V.value v2 ->
-          eval_bop op v1 v2 i = Some v ->
-          ⟦ errs, Γ ⟧ ⊢ v1 ∈ τ1 -> ⟦ errs, Γ ⟧ ⊢ v2 ∈ τ2 -> ⟦ errs, Γ ⟧ ⊢ v ∈ τ.
-      Proof.
-        intros Γ errs op τ1 τ2 τ v1 v2 v i Hbop Hv1 Hv2 Heval Ht1 Ht2;
-        inv Hbop; unravel in *; try inv_numeric;
-        repeat assert_canonical_forms;
-        try (inv_numeric_width; assert_canonical_forms);
-        try (inv Heval; auto 2; assumption).
-      Qed.
-
-      Lemma eval_member_types : forall errs Γ x v v' ts τ τ',
-          eval_member x v = Some v' ->
-          V.value v ->
-          member_type ts τ ->
-          F.get x ts = Some τ' ->
-          ⟦ errs, Γ ⟧ ⊢ v ∈ τ ->
-          ⟦ errs, Γ ⟧ ⊢ v' ∈ τ'.
-      Proof.
-        intros errs Γ x v v' ts τ τ' Heval Hv Hmem Hget Ht;
-        inv Hmem; assert_canonical_forms.
-        - eapply F.relfs_get_r in H1 as [[? ?] [? ?]]; eauto 2;
-          unravel in *; rewrite H in Heval;
-          unravel in *; inv Heval; intuition.
-        - eapply F.relfs_get_r in H6 as [[? ?] [? ?]]; eauto 2;
-          unravel in *; rewrite H in Heval;
-          unravel in *; inv Heval; intuition.
-      Qed.
-
-      Local Hint Constructors proper_nesting : core.
-      Hint Rewrite repeat_length.
-      Local Hint Resolve proper_inside_header_nesting : core.
-      Local Hint Resolve BitArith.bound0 : core.
-      Local Hint Resolve IntArith.bound0 : core.
-      Local Hint Constructors error_ok : core.
-
-      Lemma edefault_types : forall errs Γ i τ,
-          PT.proper_nesting τ ->
-          let e := edefault i τ in
-          ⟦ errs, Γ ⟧ ⊢ e ∈ τ.
-      Proof.
-        intros; subst e; induction τ using custom_t_ind; unravel;
-        invert_proper_nesting; auto 2;
-        constructor; autorewrite with core; auto 2;
-        try (apply repeat_Forall; constructor; auto 2);
-        try (ind_list_Forall; repeat inv_Forall_cons; constructor; intuition);
-        try (ind_list_predfs; repeat invert_cons_predfs; constructor;
-             try split; unravel; intuition).
-      Qed.
-
-      Local Hint Resolve Forall_impl : core.
-      Local Hint Resolve Forall_firstn : core.
-      Local Hint Resolve Forall_skipn : core.
-      Local Hint Resolve proper_inside_header_nesting : core.
-      Local Hint Resolve edefault_types : core.
-      Hint Rewrite app_length.
-      Hint Rewrite Forall_app.
-      Hint Rewrite firstn_length_le.
-      Hint Rewrite skipn_length.
-      Hint Rewrite map_length.
-      Hint Rewrite (@F.predfs_data_map string).
-      Hint Rewrite @F.map_fst.
-      Hint Rewrite @map_compose.
-      Hint Rewrite (@Forall2_map_l E.t).
-      Hint Rewrite (@Forall2_Forall E.t).
-      Hint Rewrite (@F.predfs_data_map).
-      Hint Rewrite @F.relfs_split_map_iff.
-      Hint Rewrite @F.map_snd.
-
-      Lemma eval_uop_types : forall errs Γ op e v τ τ',
-          uop_type op τ τ' -> V.value e -> eval_uop op e = Some v ->
-          ⟦ errs, Γ ⟧ ⊢ e ∈ τ -> ⟦ errs, Γ ⟧ ⊢ v ∈ τ'.
-      Proof.
-        intros errs Γ op e v τ τ' Huop Hev Heval Het;
-        inv Huop; try inv_numeric;
-        assert_canonical_forms; unravel in *;
-        inv Heval; auto 2; invert_proper_nesting;
-        repeat match goal with
-               | H: (if ?b then _ else _) = Some _
-                 |- _ => destruct b as [? | ?] eqn:?
-               | H: Some _ = Some _ |- _ => inv H
-               end; eauto 2;
-        try constructor; auto 2; try (destruct n; lia);
-        autorewrite with core; try lia;
-        try split; auto 2;
-        try (apply repeat_Forall; constructor; auto 2;
-             autorewrite with core in *; split; [intuition | unravel; eauto 5]).
-        - eapply Forall_nth_error in H9; eauto 1; simpl in *; auto 1.
-      Qed.
-    End HelpersType.
-
-    Section HelpersExist.
-      Import V.CanonicalForms.
-
-      Lemma eval_slice_exists : forall errs Γ v τ hi lo w,
-        V.value v ->
-        (lo <= hi < w)%positive ->
-        numeric_width w τ ->
-        ⟦ errs, Γ ⟧ ⊢ v ∈ τ ->
-        exists v', eval_slice hi lo v = Some v'.
-      Proof.
-        intros errs Γ v τ hi lo w Hv Hw Hnum Ht;
-        inv Hnum; assert_canonical_forms; unravel; eauto 2.
-      Qed.
-
-      Lemma eval_cast_exists : forall errs Γ e τ τ',
-        V.value e ->
-        proper_cast τ τ' ->
-        ⟦ errs, Γ ⟧ ⊢ e ∈ τ ->
-        exists v, eval_cast τ' e = Some v.
-      Proof.
-        intros ? ? ? ? ? Hv Hpc Het; inv Hpc; assert_canonical_forms;
-          unravel; simpl in *; eauto 2.
-        - destruct x; eauto 2.
-        - destruct x; eauto 2; destruct p; eauto 2;
-          try (cbv in H0; destruct H0; try destruct p; discriminate).
-        - destruct w; eauto 2.
-        - destruct w2; eauto 2.
-      Qed.
-
-      Lemma eval_bop_exists : forall errs Γ op τ1 τ2 τ (i : tags_t) v1 v2,
-          bop_type op τ1 τ2 τ ->
-          V.value v1 -> V.value v2 ->
-          ⟦ errs, Γ ⟧ ⊢ v1 ∈ τ1 -> ⟦ errs, Γ ⟧ ⊢ v2 ∈ τ2 ->
-          exists v, eval_bop op v1 v2 i = Some v.
-      Proof.
-        intros errs Γ op τ1 τ2 τ i v1 v2 Hbop Hv1 Hv2 Ht1 Ht2;
-        inv Hbop; try inv_numeric; try inv_numeric_width;
-        repeat assert_canonical_forms; unravel; eauto 2.
-      Qed.
-
-      Lemma eval_uop_exists : forall op errs Γ e τ τ',
-          uop_type op τ τ' -> V.value e -> ⟦ errs, Γ ⟧ ⊢ e ∈ τ ->
-          exists v, eval_uop op e = Some v.
-      Proof.
-        intros op errs Γ e τ τ' Hu Hv Het; inv Hu;
-        try inv_numeric; assert_canonical_forms;
-        unravel; eauto 2.
-        - assert (Hnihs : (Z.to_nat x0 < length x)%nat) by lia.
-          pose proof nth_error_exists _ _ Hnihs as [? Hnth].
-          rewrite Hnth; eauto 2.
-        - destruct (lt_dec (Pos.to_nat p) (Pos.to_nat n)) as [? | ?]; eauto 2.
-        - destruct (lt_dec (Pos.to_nat p) (Pos.to_nat n)) as [? | ?]; eauto 2.
-      Qed.
-
-      Lemma eval_member_exists : forall errs Γ x v ts τ τ',
-          V.value v ->
-          member_type ts τ ->
-          F.get x ts = Some τ' ->
-          ⟦ errs, Γ ⟧ ⊢ v ∈ τ ->
-          exists v', eval_member x v = Some v'.
-      Proof.
-        intros errs Γ x v ts τ τ' Hv Hmem Hget Ht;
-        inv Hmem; assert_canonical_forms; unravel.
-        - eapply F.relfs_get_r in H1 as [[? ?] [? ?]]; eauto 2;
-          unravel in *; rewrite H; unravel; eauto 2.
-        - eapply F.relfs_get_r in H6 as [[? ?] [? ?]]; eauto 2;
-          unravel in *; rewrite H; unravel; eauto 2.
-      Qed.
-    End HelpersExist.
-
-    (** Lookup an lvalue. *)
-    Fixpoint lv_lookup (ϵ : eenv) (lv : E.e tags_t) : option (E.e tags_t) :=
-      match lv with
-      | <{ Var x:_ @ _ }> => Env.find x ϵ
-      | <{ Mem lv:_ dot x @ _ }> =>
-        (* TODO: use monadic bind. *)
-        match lv_lookup ϵ lv with
-        | Some <{ struct { fs } @ _ }>
-        | Some <{ hdr { fs } valid:=_  @ _ }> => fs ▷ F.get x >>| snd
-        | _ => None
-        end
-      | <{ Access lv[n] @ _ }> =>
-        match lv_lookup ϵ lv with
-        | Some <{ Stack vss:_[_] nextIndex:=_ @ _ }> => nth_error vss (Z.to_nat n)
-        | _ => None
-        end
-      | _ => None
-      end.
-    (**[]*)
-
-    (** Updating an lvalue in an environment. *)
-    Fixpoint lv_update (lv v : E.e tags_t) (ϵ : eenv) : eenv :=
-      match lv with
-      | <{ Var x:_ @ _ }> => !{ x ↦ v ;; ϵ }!
-      | <{ Mem lv:_ dot x @ _ }> =>
-        match lv_lookup ϵ lv with
-        | Some <{ struct { vs } @ i }>
-          => match F.get x vs with
-            | None => ϵ
-            | Some (τ,_) => lv_update lv (E.EStruct (F.update x (τ,v) vs) i) ϵ
-            end
-        | Some <{ hdr { vs } valid:=b @ i }>
-          => match F.get x vs with
-            | None => ϵ
-            | Some (τ,_) => lv_update lv (E.EHeader (F.update x (τ,v) vs) b i) ϵ
-            end
-        | _ => ϵ
-        end
-      | <{ Access lv[n] @ _ }> =>
-        match lv_lookup ϵ lv with
-        | Some <{ Stack vss:ts[size] nextIndex:=ni @ i }> =>
-          let vss := nth_update (Z.to_nat n) v vss in
-          lv_update lv <{ Stack vss:ts[size] nextIndex:=ni @ i }> ϵ
-        | _ => ϵ
-        end
-      | _ => ϵ
-      end.
-    (**[]*)
-
-    (** Create a new environment
-        from a closure environment where
-        values of [In] args are substituted
-        into the function parameters. *)
-    Definition copy_in
-               (argsv : E.args tags_t)
-               (ϵcall : eenv) : eenv -> eenv :=
-      F.fold (fun x arg ϵ =>
-                match arg with
-                | P.PAIn (_,v)     => !{ x ↦ v ;; ϵ }!
-                | P.PAInOut (_,lv) => match lv_lookup ϵcall lv with
-                                     | None   => ϵ
-                                     | Some v => !{ x ↦ v ;; ϵ }!
-                                     end
-                | P.PAOut _    => ϵ
-                end) argsv.
-    (**[]*)
-
-    (** Update call-site environment with
-        out variables from function call evaluation. *)
-    Definition copy_out
-               (argsv : E.args tags_t)
-               (ϵf : eenv) : eenv -> eenv :=
-      F.fold (fun x arg ϵ =>
-                match arg with
-                | P.PAIn _ => ϵ
-                | P.PAOut (_,lv)
-                | P.PAInOut (_,lv) =>
-                  match Env.find x ϵf with
-                  | None   => ϵ
-                  | Some v => lv_update lv v ϵ
-                  end
-                end) argsv.
-    (**[]*)
-
-    (** Table environment. *)
-    Definition tenv : Type := Env.t string (CD.table tags_t).
-
-    (** Function declarations and closures. *)
-    Inductive fdecl : Type :=
-    | FDecl (closure : eenv) (fs : fenv) (ins : ienv) (body : ST.s tags_t)
-    with fenv : Type :=
-    | FEnv (fs : Env.t string fdecl)
-    (** Action declarations and closures *)
-    with adecl : Type :=
-    | ADecl (closure : eenv) (fs : fenv) (ins : ienv) (aa : aenv) (body : ST.s tags_t)
-    with aenv : Type :=
-    | AEnv (aa : Env.t string adecl)
-    (** Instances and Environment. *)
-    with inst : Type :=
-    | CInst (closure : eenv) (fs : fenv) (ins : ienv)
-            (tbls : tenv) (aa : aenv)
-            (apply_blk : ST.s tags_t)  (* control instance *)
-    | PInst (* TODO: parser instance *)
-    | EInst (* TODO: extern object instance *)
-    with ienv : Type :=
-    | IEnv (ins : Env.t string inst).
-    (**[]*)
-
-    (** Function lookup. *)
-    Definition lookup '(FEnv fs : fenv) : string -> option fdecl := fun s => Env.find s fs.
-
-    (** Bind a function declaration to an environment. *)
-    Definition update '(FEnv fs : fenv) (x : string) (d : fdecl) : fenv :=
-      FEnv !{ x ↦ d ;; fs }!.
-    (**[]*)
-
-    (** Instance lookup. *)
-    Definition ilookup '(IEnv fs : ienv) : string -> option inst := fun i => Env.find i fs.
-
-    (** Bind an instance to an environment. *)
-    Definition iupdate '(IEnv fs : ienv) (x : string) (d : inst) : ienv :=
-      IEnv !{ x ↦ d ;; fs }!.
-    (**[]*)
-
-    (** Action lookup. *)
-    Definition alookup '(AEnv aa : aenv) : string -> option adecl := (fun x => Env.find x aa).
-
-    (** Bind a function declaration to an environment. *)
-    Definition aupdate '(AEnv aa : aenv) (x : string) (d : adecl) : aenv :=
-      AEnv !{ x ↦ d ;; aa }!.
-    (**[]*)
-
-    (** Control plane table entries,
-        essentially mapping tables to an action call. *)
-    Definition entries : Type :=
-      list (E.e tags_t * E.matchkind) ->
-      list string ->
-      string * E.args tags_t.
-    (**[]*)
-
-    (** Control plane configuration. *)
-    Definition ctrl : Type := Env.t string entries.
-
-    (** Control declarations and closures. *)
-    Inductive cdecl : Type :=
-    | CDecl (cs : cenv) (closure : eenv) (fs : fenv) (ins : ienv)
-            (body : CD.d tags_t) (apply_block : ST.s tags_t)
-    with cenv : Type :=
-    | CEnv (cs : Env.t string cdecl).
-    (**[]*)
-
-    (** Control lookup. *)
-    Definition clookup '(CEnv cs : cenv) : string -> option cdecl := (fun x => Env.find x cs).
-
-    (** Bind an instance to an environment. *)
-    Definition cupdate '(CEnv cs : cenv) (x : string) (d : cdecl) : cenv :=
-      CEnv !{ x ↦ d ;; cs }!.
-    (**[]*)
-
-    (** Continuation statements. *)
-    Inductive kstmt : Type :=
-    | KStop                              (* end of continuation *)
-    | KSeq (s : ST.s tags_t) (k : kstmt) (* sequencing/composition *)
-    | KBlock (ϵ : eenv) (k : kstmt)      (* block: enclosing environment & continuation *)
-    | KCall (args : E.arrowE tags_t)
-            (ϵ : eenv) (k : kstmt)       (* function/procedure
-                                            call-site with arguments,
-                                            enclosing environment, & continuation *)
-    | KExit (k : kstmt)                  (* exit statement control-flow *)
-    | KReturn (o : option (E.e tags_t))
-              (k : kstmt)                (* return statement control-flow *).
-    (**[]*)
-  End StepDefs.
+  (** Continuation statements. *)
+  Inductive kstmt {tags_t : Type} : Type :=
+  | KStop                              (* end of continuation *)
+  | KSeq (s : ST.s tags_t) (k : kstmt) (* sequencing/composition *)
+  | KBlock (ϵ : @eenv tags_t) (k : kstmt)      (* block: enclosing environment & continuation *)
+  | KCall (args : E.arrowE tags_t)
+          (ϵ : @eenv tags_t) (k : kstmt)       (* function/procedure
+                                          call-site with arguments,
+                                          enclosing environment, & continuation *)
+  | KExit (k : kstmt)                  (* exit statement control-flow *)
+  | KReturn (o : option (E.e tags_t))
+            (k : kstmt)                (* return statement control-flow *).
+  (**[]*)
 
   Notation "'k{' s '}k'" := s (s custom p4kstmt at level 99).
   Notation "( x )" := x (in custom p4kstmt, x at level 99).
@@ -922,25 +46,25 @@ Module Step.
          (in custom p4kstmt at level 99, env custom p4env,
              k custom p4kstmt, right associativity).
   Notation "'EXIT' k"
-           := (KExit k)
-                (in custom p4kstmt at level 99,
-                    k custom p4kstmt, right associativity).
+    := (KExit k)
+         (in custom p4kstmt at level 99,
+             k custom p4kstmt, right associativity).
   Notation "'RETURN' o k"
-           := (KReturn o k)
-                (in custom p4kstmt at level 99,
-                    k custom p4kstmt, right associativity).
+    := (KReturn o k)
+         (in custom p4kstmt at level 99,
+             k custom p4kstmt, right associativity).
   Notation "'VOID' k"
-           := (KReturn None k)
-                (in custom p4kstmt at level 99,
-                    k custom p4kstmt, right associativity).
+    := (KReturn None k)
+         (in custom p4kstmt at level 99,
+             k custom p4kstmt, right associativity).
   Notation "'FRUIT' e k"
-           := (KReturn (Some e) k)
-                (in custom p4kstmt at level 99,
-                    k custom p4kstmt, right associativity).
-
+    := (KReturn (Some e) k)
+         (in custom p4kstmt at level 99,
+             k custom p4kstmt, right associativity).
+  
   Reserved Notation "'ℵ' env , e1 '-->' e2"
            (at level 40, e1 custom p4expr, e2 custom p4expr).
-
+  
   (** Expression evaluation. *)
   Inductive expr_step {tags_t : Type} (ϵ : eenv)
     : E.e tags_t -> E.e tags_t -> Prop :=
@@ -951,102 +75,103 @@ Module Step.
   | step_slice (e e' : E.e tags_t) (τ : E.t)
                (hi lo : positive) (i : tags_t) :
       ℵ ϵ, e -->  e' ->
-      ℵ ϵ, Slice e:τ [hi:lo] @ i -->  Slice e':τ [hi:lo] @ i
+           ℵ ϵ, Slice e:τ [hi:lo] @ i -->  Slice e':τ [hi:lo] @ i
   | step_slice_eval (v v' : E.e tags_t) (τ : E.t)
                     (hi lo : positive) (i : tags_t) :
       eval_slice hi lo v = Some v' ->
-      V.value v ->
+      value v ->
       ℵ ϵ, Slice v:τ [hi:lo] @ i -->  v'
   | step_cast (τ : E.t) (e e' : E.e tags_t) (i : tags_t) :
       ℵ ϵ, e -->  e' ->
-      ℵ ϵ, Cast e:τ @ i -->  Cast e':τ @ i
+           ℵ ϵ, Cast e:τ @ i -->  Cast e':τ @ i
   | step_cast_eval (τ : E.t) (v v' : E.e tags_t) (i : tags_t) :
       eval_cast τ v = Some v' ->
-      V.value v ->
+      value v ->
       ℵ ϵ, Cast v:τ @ i -->  v'
   | step_uop (op : E.uop) (τ : E.t)
              (e e' : E.e tags_t) (i : tags_t) :
       ℵ ϵ, e -->  e' ->
-      ℵ ϵ, UOP op e:τ @ i -->  UOP op e':τ @ i
+           ℵ ϵ, UOP op e:τ @ i -->  UOP op e':τ @ i
   | step_uop_eval (op : E.uop) (τ : E.t)
                   (v v' : E.e tags_t) (i : tags_t) :
       eval_uop op v = Some v' ->
-      V.value v ->
+      value v ->
       ℵ ϵ, UOP op v:τ @ i -->  v'
   | step_bop_l (op : E.bop) (τl τr : E.t)
                (el el' er : E.e tags_t) (i : tags_t) :
       ℵ ϵ, el -->  el' ->
-      ℵ ϵ, BOP el:τl op er:τr @ i -->  BOP el':τl op er:τr @ i
+           ℵ ϵ, BOP el:τl op er:τr @ i -->  BOP el':τl op er:τr @ i
   | step_bop_r (op : E.bop) (τl τr : E.t)
                (vl er er' : E.e tags_t) (i : tags_t) :
-      V.value vl ->
+      value vl ->
       ℵ ϵ, er -->  er' ->
-      ℵ ϵ, BOP vl:τl op er:τr @ i -->  BOP vl:τl op er':τr @ i
+           ℵ ϵ, BOP vl:τl op er:τr @ i -->  BOP vl:τl op er':τr @ i
   | step_bop_eval (op : E.bop) (τl τr : E.t)
                   (vv vl vr : E.e tags_t) (i : tags_t) :
       eval_bop op vl vr i = Some vv ->
-      V.value vl -> V.value vr ->
+      value vl -> value vr ->
       ℵ ϵ, BOP vl:τl op vr:τr @ i -->  vv
   | step_member (x : string) (τ : E.t)
                 (e e' : E.e tags_t) (i : tags_t) :
       ℵ ϵ, e -->  e' ->
-      ℵ ϵ, Mem e:τ dot x @ i -->  Mem e:τ dot x @ i
+           ℵ ϵ, Mem e:τ dot x @ i -->  Mem e:τ dot x @ i
   | step_member_eval (x : string) (τ : E.t)
                      (v v' : E.e tags_t) (i : tags_t) :
       eval_member x v = Some v' ->
-      V.value v ->
+      value v ->
       ℵ ϵ, Mem v:τ dot x @ i -->  v'
   | step_stack_access (e e' : E.e tags_t) (n : Z) (i : tags_t) :
       ℵ ϵ, e -->  e' ->
-      ℵ ϵ, Access e[n] @ i -->  Access e'[n] @ i
+           ℵ ϵ, Access e[n] @ i -->  Access e'[n] @ i
   | step_stack_access_eval (v v' : E.e tags_t) (n : Z) (i : tags_t) :
       header_stack_data v >>| fourple_4 >>=
-                 (fun hs => nth_error hs (Z.to_nat n)) = Some v' ->
-      V.value v ->
+                        (fun hs => nth_error hs (Z.to_nat n)) = Some v' ->
+      value v ->
       ℵ ϵ, Access v[n] @ i -->  v'
   | step_tuple (prefix suffix : list (E.e tags_t))
                (e e' : E.e tags_t) (i : tags_t) :
-      Forall V.value prefix ->
+      Forall value prefix ->
       ℵ ϵ, e -->  e' ->
-      let es := prefix ++ e :: suffix in
-      let es' := prefix ++ e' :: suffix in
-      ℵ ϵ, tup es @ i -->  tup es' @ i
+           let es := prefix ++ e :: suffix in
+           let es' := prefix ++ e' :: suffix in
+           ℵ ϵ, tup es @ i -->  tup es' @ i
   | step_struct (prefix suffix : F.fs string (E.t * E.e tags_t))
                 (x : string) (τ : E.t)
                 (e e' : E.e tags_t) (i : tags_t) :
-      F.predfs_data (V.value ∘ snd) prefix ->
+      F.predfs_data (value ∘ snd) prefix ->
       ℵ ϵ, e -->  e' ->
-      let fs := prefix ++ (x,(τ,e)) :: suffix in
-      let fs' := prefix ++ (x,(τ,e')) :: suffix in
-      ℵ ϵ, struct { fs } @ i -->  struct { fs' } @ i
+           let fs := prefix ++ (x,(τ,e)) :: suffix in
+           let fs' := prefix ++ (x,(τ,e')) :: suffix in
+           ℵ ϵ, struct { fs } @ i -->  struct { fs' } @ i
   | step_header (prefix suffix : F.fs string (E.t * E.e tags_t))
                 (x : string) (τ : E.t)
                 (b e e' : E.e tags_t) (i : tags_t) :
-      V.value b ->
-      F.predfs_data (V.value ∘ snd) prefix ->
+      value b ->
+      F.predfs_data (value ∘ snd) prefix ->
       ℵ ϵ, e -->  e' ->
-      let fs := prefix ++ (x,(τ,e)) :: suffix in
-      let fs' := prefix ++ (x,(τ,e')) :: suffix in
-      ℵ ϵ, hdr { fs } valid:=b @ i -->  hdr { fs' } valid:=b @ i
+           let fs := prefix ++ (x,(τ,e)) :: suffix in
+           let fs' := prefix ++ (x,(τ,e')) :: suffix in
+           ℵ ϵ, hdr { fs } valid:=b @ i -->  hdr { fs' } valid:=b @ i
   | step_header_valid (fs : F.fs string (E.t * E.e tags_t))
                       (e e' : E.e tags_t) (i : tags_t) :
       ℵ ϵ, e -->  e' ->
-      ℵ ϵ, hdr { fs } valid:=e @ i -->  hdr { fs } valid:=e' @ i
+           ℵ ϵ, hdr { fs } valid:=e @ i -->  hdr { fs } valid:=e' @ i
   | step_header_stack (ts : F.fs string (E.t))
                       (prefix suffix : list (E.e tags_t))
                       (e e' : E.e tags_t) (size : positive)
                       (ni : Z) (i : tags_t) :
-      Forall V.value prefix ->
+      Forall value prefix ->
       ℵ ϵ, e -->  e' ->
-      let hs := prefix ++ e :: suffix in
-      let hs' := prefix ++ e' :: suffix in
-      ℵ ϵ, Stack hs:ts[size] nextIndex:=ni @ i -->  Stack hs':ts[size] nextIndex:=ni @ i
+           let hs := prefix ++ e :: suffix in
+           let hs' := prefix ++ e' :: suffix in
+           ℵ ϵ, Stack hs:ts[size] nextIndex:=ni @ i -->
+           Stack hs':ts[size] nextIndex:=ni @ i
   where "'ℵ' ϵ , e1 '-->' e2" := (expr_step ϵ e1 e2).
   (**[]*)
 
   Reserved Notation "'ℶ' e1 '-->'  e2"
            (at level 40, e1 custom p4expr, e2 custom p4expr).
-
+  
   Inductive lvalue_step {tags_t : Type} : E.e tags_t -> E.e tags_t -> Prop :=
   | lstep_member (e e' : E.e tags_t) (τ : E.t) (x : string) (i : tags_t) :
       ℶ e -->  e' ->
@@ -1056,19 +181,19 @@ Module Step.
       ℶ Access e[idx] @ i -->   Access e'[idx] @ i
   where "'ℶ' e1 '-->' e2" := (lvalue_step e1 e2).
   (**[]*)
-
+  
   Reserved Notation "'π' envn , pe1 '-->' pe2"
            (at level 40, pe1 custom p4prsrexpr, pe2 custom p4prsrexpr).
-
+  
   Inductive step_parser_expr {tags_t : Type} (ϵ : @eenv tags_t)
     : PR.e tags_t -> PR.e tags_t -> Prop :=
   | step_select_discriminee (e e' : E.e tags_t) (d : PR.e tags_t)
                             (cases : F.fs PR.pat (PR.e tags_t)) (i : tags_t) :
       ℵ ϵ, e -->  e' ->
-      π ϵ, select e { cases } default:=d @ i-->  select e' { cases } default:=d @ i
+           π ϵ, select e { cases } default:=d @ i-->  select e' { cases } default:=d @ i
   | step_select_resolve (v : E.e tags_t) (d : PR.e tags_t)
                         (cases : F.fs PR.pat (PR.e tags_t)) (i : tags_t) :
-      V.value v ->
+      value v ->
       let pe := match F.find_value (fun _ => false) cases with (** TODO!! *)
                 | None => d
                 | Some pe => pe
@@ -1080,32 +205,32 @@ Module Step.
   Reserved Notation "'ℸ' cfg , tbls , aa , fns , ins , ϵ1 , k1 '-->' k2 , ϵ2"
            (at level 40, k1 custom p4kstmt, k2 custom p4kstmt,
             ϵ1 custom p4env, ϵ2 custom p4env).
-(** TODO: Architecture & Target Issues:
-    - Need a general model for architectures & targets that is both:
-      + suitably abstract & parameterizable for all levels of compilation.
-      + constrained enough to be useful in dynamic semantics.
-    - Unsure of how to evaluate externs.
-    - Unsure of packet representation.
-    - Unsure of how to represent & evaluate pipeline.
-    ```p4
-    extern packet_in {
-        void extract<T>(out T); /// reads from packet into out var
-        T lookahead<T>(); /// reads from packet
-        void advance(in bit<32>); /// writes to packet cursor
-        bit<32> length(); /// reads from packet
-    }
+  (** TODO: Architecture & Target Issues:
+      - Need a general model for architectures & targets that is both:
+        + suitably abstract & parameterizable for all levels of compilation.
+        + constrained enough to be useful in dynamic semantics.
+      - Unsure of how to evaluate externs.
+      - Unsure of packet representation.
+      - Unsure of how to represent & evaluate pipeline.
+      ```p4
+      extern packet_in {
+      void extract<T>(out T); /// reads from packet into out var
+      T lookahead<T>(); /// reads from packet
+      void advance(in bit<32>); /// writes to packet cursor
+      bit<32> length(); /// reads from packet
+      }
 
-    extern packet_out {
-           void emit<T>(in T); /// writes to output packet
-    }
-    ```
-    Brain storm: could extern methods just be coq-functions?
-    Since they are purely semantic, do I even need a consistent
-    representation?
+     extern packet_out {
+            void emit<T>(in T); /// writes to output packet
+     }
+     ```
+     Brain storm: could extern methods just be coq-functions?
+     Since they are purely semantic, do I even need a consistent
+     representation?
 
-    Perhaps all IRs share some notion of "packet",
-    and each IR may deal with extern-representations separately?
- *)
+     Perhaps all IRs share some notion of "packet",
+     and each IR may deal with extern-representations separately?
+   *)
 
   (** Statement evaluation.
       This continuation-based approach
@@ -1134,13 +259,13 @@ Module Step.
       ℸ cfg, tbls, aa, fns, ins, ϵ,
       κ asgn e1 := e2:τ @ i ⋅ k -->  κ asgn e1 := e2':τ @ i ⋅ k, ϵ
   | step_asgn_l (e1 e1' v2 : E.e tags_t) (τ : E.t) (i : tags_t) (k : kstmt) :
-      V.value v2 ->
+      value v2 ->
       ℶ e1 -->  e1' ->
       ℸ cfg, tbls, aa, fns, ins, ϵ,
       κ asgn e1 := v2:τ @ i ⋅ k -->  κ asgn e1' := v2:τ @ i ⋅ k, ϵ
   | step_asgn (v1 v2 : E.e tags_t) (τ : E.t) (i : tags_t) (k : kstmt) :
-      V.lvalue v1 ->
-      V.value v2 ->
+      lvalue v1 ->
+      value v2 ->
       let ϵ' := lv_update v1 v2 ϵ in
       ℸ cfg, tbls, aa, fns, ins, ϵ, κ asgn v1 := v2:τ @ i ⋅ k -->  k, ϵ'
   | step_exit (i : tags_t) (k : kstmt) :
@@ -1156,7 +281,7 @@ Module Step.
       ℸ cfg, tbls, aa, fns, ins, ϵ,
       κ return e:τ @ i ⋅ k -->  κ return e':τ @ i ⋅ k, ϵ
   | step_return_value (v : E.e tags_t) (τ : E.t) (i : tags_t) (k : kstmt) :
-      V.value v ->
+      value v ->
       ℸ cfg, tbls, aa, fns, ins, ϵ,
       κ return v:τ @ i ⋅ k -->  FRUIT v k, ϵ
   | step_kreturn_kseq (o : option (E.e tags_t)) (s : ST.s tags_t) (k : kstmt) :
@@ -1180,7 +305,7 @@ Module Step.
                         (i : tags_t) (k : kstmt) :
       F.predfs_data
         (P.pred_paramarg
-           (V.value ∘ snd) (V.lvalue ∘ snd)) prefix ->
+           (value ∘ snd) (lvalue ∘ snd)) prefix ->
       ℵ ϵ, e -->  e' ->
       let args  := prefix ++ (x, P.PAIn (τ,e))  :: suffix in
       let args' := prefix ++ (x, P.PAIn (τ,e')) :: suffix in
@@ -1191,7 +316,7 @@ Module Step.
                          (e e' : E.e tags_t) (i : tags_t) (k : kstmt) :
        F.predfs_data
          (P.pred_paramarg
-            (V.value ∘ snd) (V.lvalue ∘ snd)) args ->
+            (value ∘ snd) (lvalue ∘ snd)) args ->
        ℶ e -->  e' ->
        ℸ cfg, tbls, aa, fns, ins, ϵ,
        κ let e:τ  := call f with args @ i ⋅ k -->
@@ -1202,10 +327,10 @@ Module Step.
                   (body : ST.s tags_t) (fϵ : eenv)
                   (fclosure : fenv) (fins : ienv) :
        lookup fns f = Some (FDecl fϵ fclosure fins body) ->
-       predop (V.lvalue ∘ snd) o ->
+       predop (lvalue ∘ snd) o ->
        F.predfs_data
          (P.pred_paramarg
-            (V.value ∘ snd) (V.lvalue ∘ snd)) args ->
+            (value ∘ snd) (lvalue ∘ snd)) args ->
        let fϵ' := copy_in args ϵ fϵ in
        let arrow := P.Arrow args o in
        ℸ cfg, tbls, aa, fns, ins, ϵ,
