deps/poulet4/lib/P4cub/BigStep/BSIndPrincip.v
@@ -1,0 +1,264 @@
+Set Warnings "-custom-entry-overridden".
+Require Import
+        Poulet4.P4cub.Envn
+        Poulet4.P4cub.Syntax.AST
+        Poulet4.P4cub.BigStep.Value
+        Poulet4.P4cub.BigStep.BSUtil
+        Poulet4.P4cub.BigStep.BSSemantics
+        Poulet4.P4cub.BigStep.ValueAux
+        Coq.ZArith.BinInt.
+Import Step P.P4cubNotations Val.ValueNotations.
+
+(** A custom induction principle for
+    the expression big-step relation. *)
+Section ExprEvalInduction.
+  Variable (tags_t: Type).
+  
+  Variable P : epsilon -> E.e tags_t -> V.v -> Prop.
+  
+  Hypothesis HBool : forall ϵ b i, P ϵ <{ BOOL b @ i }> ~{ VBOOL b }~.
+  
+  Hypothesis HBit : forall ϵ w n i, P ϵ <{ w W n @ i }> ~{ w VW n }~.
+  
+  Hypothesis HInt : forall ϵ w z i, P ϵ <{ w S z @ i }> ~{ w VS z }~.
+  
+  Hypothesis HVar : forall ϵ x τ i v,
+      Env.find x ϵ = Some v ->
+      P ϵ <{ Var x:τ @ i }> v.
+  (**[]*)
+  
+  Hypothesis HSlice : forall ϵ e τ hi lo i v v',
+      eval_slice hi lo v = Some v' ->
+      ⟨ ϵ, e ⟩ ⇓ v ->
+      P ϵ e v ->
+      P ϵ <{ Slice e:τ [hi:lo] @ i }> v'.
+  (**[]*)
+  
+  Hypothesis HCast : forall ϵ τ e i v v',
+      eval_cast τ v = Some v' ->
+      ⟨ ϵ, e ⟩ ⇓ v ->
+      P ϵ e v ->
+      P ϵ <{ Cast e:τ @ i }> v'.
+  (**[]*)
+  
+  Hypothesis HError : forall ϵ err i, P ϵ <{ Error err @ i }> ~{ ERROR err }~.
+  
+  Hypothesis HMatchkind : forall ϵ mk i,
+      P ϵ <{ Matchkind mk @ i }> ~{ MATCHKIND mk }~.
+  (**[]*)
+  
+  Hypothesis HUop : forall ϵ op τ e i v v',
+      eval_uop op v = Some v' ->
+      ⟨ ϵ, e ⟩ ⇓ v ->
+      P ϵ e v ->
+      P ϵ <{ UOP op e:τ @ i }> v'.
+  
+  Hypothesis HBop : forall ϵ op τ1 τ2 e1 e2 i v v1 v2,
+      eval_bop op v1 v2 = Some v ->
+      ⟨ ϵ, e1 ⟩ ⇓ v1 ->
+      P ϵ e1 v1 ->
+      ⟨ ϵ, e2 ⟩ ⇓ v2 ->
+      P ϵ e2 v2 ->
+      P ϵ <{ BOP e1:τ1 op e2:τ2 @ i }> v.
+  (**[]*)
+  
+  Hypothesis HMem : forall ϵ e x τ i v v',
+      eval_member x v = Some v' ->
+      ⟨ ϵ, e ⟩ ⇓ v ->
+      P ϵ e v ->
+      P ϵ <{ Mem e:τ dot x @ i }> v'.
+  (**[]*)
+  
+  Hypothesis HTuple : forall ϵ es i vs,
+      Forall2 (fun e v => ⟨ ϵ, e ⟩ ⇓ v) es vs ->
+      Forall2 (P ϵ) es vs ->
+      P ϵ <{ tup es @ i }> ~{ TUPLE vs }~.
+  (**[]*)
+  
+  Hypothesis HStructLit : forall ϵ efs i vfs,
+      F.relfs
+        (fun te v =>
+           let e := snd te in ⟨ ϵ, e ⟩ ⇓ v) efs vfs ->
+      F.relfs (fun te v => let e := snd te in P ϵ e v) efs vfs ->
+      P ϵ <{ struct { efs } @ i }> ~{ STRUCT { vfs } }~.
+  (**[]*)
+  
+  Hypothesis HHdrLit : forall ϵ efs e i b vfs,
+      F.relfs
+        (fun te v =>
+           let e := snd te in ⟨ ϵ, e ⟩ ⇓ v) efs vfs ->
+      F.relfs (fun te v => let e := snd te in P ϵ e v) efs vfs ->
+      ⟨ ϵ, e ⟩ ⇓ VBOOL b ->
+      P ϵ e ~{ VBOOL b }~ ->
+      P ϵ <{ hdr { efs } valid:=e @ i }> ~{ HDR { vfs } VALID:=b }~.
+  (**[]*)
+  
+  Hypothesis HHdrStack : forall ϵ ts hs n ni i vss,
+      Forall2
+        (fun e bvs =>
+           let b := fst bvs in
+           let vs := snd bvs in
+           ⟨ ϵ, e ⟩ ⇓ HDR { vs } VALID:=b)
+        hs vss ->
+      Forall2
+        (fun e bvs =>
+           let b := fst bvs in
+           let vs := snd bvs in
+           P ϵ e ~{ HDR { vs } VALID:=b}~ )
+        hs vss ->
+      P ϵ <{ Stack hs:ts[n] nextIndex:=ni @ i }> ~{ STACK vss:ts[n] NEXT:=ni }~.
+  (**[]*)
+  
+  Hypothesis HAccess : forall ϵ e i n index ni ts vss b vs,
+      nth_error vss (Z.to_nat index) = Some (b,vs) ->
+      ⟨ ϵ, e ⟩ ⇓ STACK vss:ts[n] NEXT:=ni ->
+                                       P ϵ e ~{ STACK vss:ts[n] NEXT:=ni }~ ->
+                                       P ϵ <{ Access e[index] @ i }> ~{ HDR { vs } VALID:=b }~.
+  (**[]*)
+  
+  (** Custom induction principle for
+      the expression big-step relation.
+      [Do induction ?H using custom_expr_big_step_ind]. *)
+  Definition custom_expr_big_step_ind :
+    forall (ϵ : epsilon) (e : E.e tags_t)
+      (v : V.v) (Hy : ⟨ ϵ, e ⟩ ⇓ v), P ϵ e v :=
+    fix ebsind ϵ e v Hy :=
+      let fix lind
+              {es : list (E.e tags_t)}
+              {vs : list (V.v)}
+              (HR : Forall2 (fun e v => ⟨ ϵ, e ⟩ ⇓ v) es vs)
+          : Forall2 (P ϵ) es vs :=
+          match HR with
+          | Forall2_nil _ => Forall2_nil _
+          | Forall2_cons _ _ Hh Ht
+            => Forall2_cons _ _ (ebsind _ _ _ Hh) (lind Ht)
+          end in
+      let fix fsind
+              {efs : F.fs string (E.t * E.e tags_t)}
+              {vfs : F.fs string (V.v)}
+              (HRs : F.relfs
+                       (fun te v =>
+                          let e := snd te in
+                          ⟨ ϵ , e ⟩ ⇓ v) efs vfs)
+          : F.relfs
+              (fun te v => let e := snd te in P ϵ e v)
+              efs vfs :=
+          match HRs with
+          | Forall2_nil _ => Forall2_nil _
+          | Forall2_cons _ _ (conj Hx Hhd) Htl
+            => Forall2_cons _ _ (conj Hx (ebsind _ _ _ Hhd)) (fsind Htl)
+          end in
+      let fix ffind
+              {es : list (E.e tags_t)}
+              {vss : list (bool * F.fs string (V.v))}
+              (HRs : Forall2
+                       (fun e bvs =>
+                          let b := fst bvs in
+                          let vs := snd bvs in
+                          ⟨ ϵ, e ⟩ ⇓ HDR { vs } VALID:=b)
+                       es vss)
+          : Forall2
+              (fun e bvs =>
+                 let b := fst bvs in
+                 let vs := snd bvs in
+                 P ϵ e ~{ HDR { vs } VALID:=b}~ )
+              es vss :=
+          match HRs with
+          | Forall2_nil _ => Forall2_nil _
+          | Forall2_cons _ _ Hhead Htail
+            => Forall2_cons _ _ (ebsind _ _ _ Hhead) (ffind Htail)
+          end in
+      match Hy with
+      | ebs_bool _ b i => HBool ϵ b i
+      | ebs_bit _ w n i => HBit ϵ w n i
+      | ebs_int _ w z i => HInt ϵ w z i
+      | ebs_var _ _ τ i _ Hx => HVar _ _ τ i _ Hx
+      | ebs_slice _ _ _ _ _ i _ _ Hv He
+        => HSlice _ _ _ _ _ i _ _ Hv He (ebsind _ _ _ He)
+      | ebs_cast _ _ _ i _ _ Hv He
+        => HCast _ _ _ i _ _ Hv He (ebsind _ _ _ He)
+      | ebs_error _ err i => HError _ err i
+      | ebs_matchkind _ mk i => HMatchkind _ mk i
+      | ebs_uop _ _ _ _ i _ _ Hv He
+        => HUop _ _ _ _ i _ _ Hv He (ebsind _ _ _ He)
+      | ebs_bop _ _ _ _ _ _ i _ _ _ Hv He1 He2
+        => HBop _ _ _ _ _ _ i _ _ _ Hv He1 (ebsind _ _ _ He1) He2 (ebsind _ _ _ He2)
+      | ebs_mem _ _ _ _ i _ _ Heval He
+        => HMem _ _ _ _ i _ _ Heval He (ebsind _ _ _ He)
+      | ebs_tuple _ _ i _ HR => HTuple _ _ i _ HR (lind HR)
+      | ebs_struct_lit _ _ i _ HR => HStructLit _ _ i _ HR (fsind HR)
+      | ebs_hdr_lit _ _ _ i _ _ HR He
+        => HHdrLit _ _ _ i _ _ HR (fsind HR) He (ebsind _ _ _ He)
+      | ebs_hdr_stack _ _ _ n ni i _ HR
+        => HHdrStack _ _ _ n ni i _ HR (ffind HR)
+      | ebs_access _ _ i n index ni ts _ _ _ Hnth He
+        => HAccess _ _ i n index ni ts _ _ _ Hnth He (ebsind _ _ _ He)
+      end.
+  (**[]*)
+End ExprEvalInduction.
+
+Section ParserExprInduction.
+  Variable tags_t : Type.
+  Variable P : epsilon -> PR.e tags_t -> PR.state -> Prop.
+  
+  Hypothesis HGoto : forall ϵ st i,
+      P ϵ p{ goto st @ i }p st.
+  
+  Hypothesis HSelect : forall ϵ e def cases i v
+                         st_def vcases,
+      ⟨ ϵ, e ⟩ ⇓ v ->
+      Forall2
+        (fun pe ps =>
+           let p := fst pe in
+           let p' := fst ps in
+           let e := snd pe in
+           let s := snd ps in
+           p = p' /\ ⦑ ϵ, e ⦒ ⇓ s)
+        cases vcases ->
+      Forall2 (fun pe ps =>
+                 let e := snd pe in
+                 let s := snd ps in
+                 P ϵ e s) cases vcases ->
+      ⦑ ϵ, def ⦒ ⇓ st_def ->
+      P ϵ def st_def ->
+      let st := match F.find_value (fun p => match_pattern p v) vcases with
+                | None => st_def
+                | Some st => st
+                end in
+      P ϵ p{ select e { cases } default:=def @ i }p st.
+  
+  Definition custom_parser_expr_big_step_ind :
+    forall (ϵ : epsilon) (e : PR.e tags_t) (st : PR.state),
+      ⦑ ϵ, e ⦒ ⇓ st -> P ϵ e st :=
+    fix pebsind ϵ e st H :=
+      let fix cases_ind
+              {cases : F.fs PR.pat (PR.e tags_t)}
+              {vcases : F.fs PR.pat PR.state}
+              (Hcases :
+                 Forall2
+                   (fun pe ps =>
+                      let p := fst pe in
+                      let p' := fst ps in
+                      let e := snd pe in
+                      let s := snd ps in
+                      p = p' /\ ⦑ ϵ, e ⦒ ⇓ s)
+                   cases vcases)
+          : Forall2
+              (fun pe ps =>
+                 let e := snd pe in
+                 let s := snd ps in
+                 P ϵ e s) cases vcases :=
+          match Hcases with
+          | Forall2_nil _ => Forall2_nil _
+          | Forall2_cons _ _ (conj _ Hcase) Htail
+            => Forall2_cons _ _ (pebsind _ _ _ Hcase) (cases_ind Htail)
+          end in
+      match H with
+      | pebs_goto _ st i => HGoto _ st i
+      | pebs_select _ _ _ _ i _ _ _ He Hcases Hdef
+        => HSelect _ _ _ _ i _ _ _ He
+                  Hcases (cases_ind Hcases)
+                  Hdef (pebsind _ _ _ Hdef)
+      end.
+  (**[]*)
+End ParserExprInduction.
