deps/poulet4/lib/P4cub/SmallStep/SSDeterminism.v
@@ -1,11 +1,10 @@
-Require Import SSSemantics.
+Require Import SSSemantics SSValue.
 
 Module P := Poulet4.P4cub.Syntax.AST.P4cub.
 Module E := P.Expr.
 Module PR := P.Parser.
 Import P.P4cubNotations.
-Import Step.
-Import F.FieldTactics.
+Import Step F.FieldTactics.
 
 Section Determinism.
   Context {tags_t : Type}.
@@ -17,7 +16,7 @@ Section Determinism.
     Local Hint Extern 0 => inv_Forall_cons : core.
 
     Lemma step_value_false : forall ϵ (e e' : E.e tags_t),
-      ℵ ϵ, e -->  e' -> ~ V.value e.
+      ℵ ϵ, e -->  e' -> ~ value e.
     Proof.
       intros ϵ e e' He Hv; induction He; inv Hv;
       repeat subst_term; autorewrite with core in *;
@@ -27,10 +26,10 @@ Section Determinism.
 
   Ltac step_value :=
     match goal with
-    | He : (ℵ _, ?e -->  _), Hv : (V.value ?e)
+    | He : (ℵ _, ?e -->  _), Hv : (value ?e)
       |- _ => apply step_value_false in He; contradiction
     | He : (ℵ _, ?e -->  _)
-      |- ~ V.value ?e => apply step_value_false in He; assumption
+      |- ~ value ?e => apply step_value_false in He; assumption
     end.
   (**[]*)
 
@@ -56,22 +55,22 @@ Section Determinism.
       intros ϵ e e1 e2 He1; generalize dependent e2;
       induction He1; intros e2' He2'; inv He2';
       f_equal; auto 2; subst; repeat subst_term.
-      - assert (~ V.value e) by auto 1.
-        assert (~ V.value e0) by auto 1.
+      - assert (~ value e) by auto 1.
+        assert (~ value e0) by auto 1.
         eapply Forall_until_eq in H0 as [? [? ?]]; eauto 1; subst.
         repeat f_equal; auto 2.
       - unfold F.predfs_data, F.predf_data in *.
-        assert (~ (V.value ∘ snd ∘ snd) (x, (τ, e))) by (unravel; auto 1).
-        assert (~ (V.value ∘ snd ∘ snd) (x0, (τ0, e0))) by (unravel; auto 1).
+        assert (~ (value ∘ snd ∘ snd) (x, (τ, e))) by (unravel; auto 1).
+        assert (~ (value ∘ snd ∘ snd) (x0, (τ0, e0))) by (unravel; auto 1).
         eapply Forall_until_eq in H0 as [? [? ?]]; eauto 1; subst.
         repeat f_equal; inv_eq; auto 2.
       - unfold F.predfs_data, F.predf_data in *.
-        assert (~ (V.value ∘ snd ∘ snd) (x, (τ, e))) by (unravel; auto 1).
-        assert (~ (V.value ∘ snd ∘ snd) (x0, (τ0, e0))) by (unravel; auto 1).
+        assert (~ (value ∘ snd ∘ snd) (x, (τ, e))) by (unravel; auto 1).
+        assert (~ (value ∘ snd ∘ snd) (x0, (τ0, e0))) by (unravel; auto 1).
         eapply Forall_until_eq in H1 as [? [? ?]]; eauto 1; subst.
         repeat f_equal; inv_eq; auto 2.
-      - assert (~ V.value e) by auto 1.
-        assert (~ V.value e0) by auto 1.
+      - assert (~ value e) by auto 1.
+        assert (~ value e0) by auto 1.
         eapply Forall_until_eq in H1 as [? [? ?]]; eauto 1; subst.
         repeat f_equal; auto 2.
     Qed.
