deps/poulet4/lib/P4cub/SmallStep/SSValue.v
@@ -1,0 +1,260 @@
+Set Warnings "-custom-entry-overridden".
+Require Export Poulet4.P4cub.Static.Check.
+Require Import Poulet4.P4cub.Syntax.SynIndPrincip.
+
+(** * Small-Step Values *)
+
+Module P := P4cub.
+Module E := P.Expr.
+Module F := P.F.
+
+Import P.P4cubNotations.
+
+Inductive value {tags_t : Type} : E.e tags_t -> Prop :=
+| value_bool (b : bool) (i : tags_t) :
+    value <{ BOOL b @ i }>
+| value_bit (w : positive) (n : Z) (i : tags_t) :
+    value <{ w W n @ i }>
+| value_int (w : positive) (z : Z) (i : tags_t) :
+    value <{ w S z @ i }>
+| value_tuple (es : list (E.e tags_t)) (i : tags_t) :
+    Forall value es ->
+    value <{ tup es @ i }>
+| value_struct (fs : F.fs string (E.t * E.e tags_t))
+               (i : tags_t) :
+    F.predfs_data (value ∘ snd) fs ->
+    value <{ struct { fs } @ i }>
+| value_header (fs : F.fs string (E.t * E.e tags_t))
+               (b : E.e tags_t) (i : tags_t) :
+    value b ->
+    F.predfs_data (value ∘ snd) fs ->
+    value <{ hdr { fs } valid:=b @ i }>
+| value_error (err : option (string)) (i : tags_t) :
+    value <{ Error err @ i }>
+| value_matchkind (mk : E.matchkind) (i : tags_t) :
+    value <{ Matchkind mk @ i }>
+| value_headerstack (fs : F.fs string (E.t))
+                    (hs : list (E.e tags_t)) (n : positive)
+                    (ni : Z) (i : tags_t) :
+    Forall value hs ->
+    value <{ Stack hs:fs[n] nextIndex:=ni @ i }>.
+(**[]*)
+
+Section IsValueInduction.
+  Variable tags_t : Type.
+  
+  Variable P : E.e tags_t -> Prop.
+  
+  Hypothesis HBool : forall b i, P <{ BOOL b @ i }>.
+  
+  Hypothesis HBit : forall w n i, P <{ w W n @ i }>.
+  
+  Hypothesis HInt : forall w z i, P <{ w S z @ i }>.
+  
+  Hypothesis HTuple : forall es i,
+      Forall value es ->
+      Forall P es ->
+      P <{ tup es @ i }>.
+  
+  Hypothesis HStruct : forall fs i,
+      F.predfs_data (value ∘ snd) fs ->
+      F.predfs_data (P ∘ snd) fs ->
+      P <{ struct { fs } @ i }>.
+  
+  Hypothesis HHeader : forall fs b i,
+      value b ->
+      P b ->
+      F.predfs_data (value ∘ snd) fs ->
+      F.predfs_data (P ∘ snd) fs ->
+      P <{ hdr { fs } valid:=b @ i }>.
+  
+  Hypothesis HError : forall err i, P <{ Error err @ i }>.
+  
+  Hypothesis HMatchkind : forall mk i, P <{ Matchkind mk @ i }>.
+  
+  Hypothesis HStack : forall fs hs n ni i,
+      Forall value hs ->
+      Forall P hs ->
+      P <{ Stack hs:fs[n] nextIndex:=ni @ i }>.
+  
+  Definition custom_value_ind : forall (e : E.e tags_t),
+      value e -> P e :=
+    fix vind (e : E.e tags_t) (H : value e) : P e :=
+      let fix lind {es : list (E.e tags_t)}
+              (Hes : Forall value es) : Forall P es :=
+          match Hes with
+          | Forall_nil _ => Forall_nil _
+          | Forall_cons _ Hh Ht => Forall_cons _ (vind _ Hh) (lind Ht)
+          end in
+      let fix find {A : Type} {fs : F.fs string (A * E.e tags_t)}
+              (Hfs : F.predfs_data (value ∘ snd) fs) :
+            F.predfs_data (P ∘ snd) fs :=
+          match Hfs with
+          | Forall_nil _ => Forall_nil _
+          | Forall_cons _ Hh Ht => Forall_cons _ (vind _ Hh) (find Ht)
+          end in
+      match H with
+      | value_bool b i => HBool b i
+      | value_bit w n i => HBit w n i
+      | value_int w z i => HInt w z i
+      | value_tuple _ i Hes => HTuple _ i Hes (lind Hes)
+      | value_struct _ i Hfs => HStruct _ i Hfs (find Hfs)
+      | value_header _ _ i Hb Hfs
+        => HHeader _ _ i Hb (vind _ Hb) Hfs (find Hfs)
+      | value_error err i => HError err i
+      | value_matchkind mk i => HMatchkind mk i
+      | value_headerstack fs _ n ni i Hhs => HStack fs _ n ni i Hhs (lind Hhs)
+      end.
+End IsValueInduction.
+
+Section Lemmas.
+  Import F.FieldTactics.
+  
+  Hint Constructors value : core.
+  Hint Extern 0 => inv_Forall_cons : core.
+  
+  Lemma value_exm : forall {tags_t : Type} (e : E.e tags_t), value e \/ ~ value e.
+  Proof.
+    induction e using custom_e_ind; auto 2;
+      try (right; intros H'; inv H'; contradiction).
+    - assert (Forall value es \/ ~ Forall value es).
+      { ind_list_Forall; intuition. }
+      intuition. right; intros H'; inv H'. contradiction.
+    - assert (F.predfs_data (value ∘ snd) fields \/
+              ~ F.predfs_data (value ∘ snd) fields).
+      { ind_list_predfs; unfold F.predfs_data in *; intuition. }
+      intuition. right; intros H'; inv H'. contradiction.
+    - assert (F.predfs_data (value ∘ snd) fields \/
+              ~ F.predfs_data (value ∘ snd) fields).
+      { ind_list_predfs; unfold F.predfs_data in *; intuition. }
+      intuition; right; intros H'; inv H'; contradiction.
+    - assert (Forall value hs \/ ~ Forall value hs).
+      { ind_list_Forall; intuition. }
+      intuition. right; intros H'; inv H'. contradiction.
+  Qed.
+End Lemmas.
+
+Inductive lvalue {tags_t : Type} : E.e tags_t -> Prop :=
+| lvalue_var x τ i :
+    lvalue <{ Var x:τ @ i }>
+| lvalue_member lv τ x i :
+    lvalue lv ->
+    lvalue <{ Mem lv:τ dot x @ i }>
+| lvalue_access lv idx i :
+    lvalue lv ->
+    lvalue <{ Access lv[idx] @ i }>.
+(**[]*)
+
+Module CanonicalForms.
+  Ltac invert_value :=
+    match goal with
+    | H: value _ |- _ => inv H
+    end.
+  (**[]*)
+  
+  Ltac invert_expr_check :=
+    match goal with
+    | H: ⟦ _, _ ⟧ ⊢ _ ∈ _ |- _ => inv H
+    end.
+  (**[]*)
+  
+  Ltac invert_canonical := invert_value; invert_expr_check.
+  
+  Ltac crush_canonical := intros; invert_canonical; eauto 4.
+  
+  Section CanonicalForms.
+    Variable errs : errors.
+    
+    Variable Γ : gamma.
+    
+    Context {tags_t : Type}.
+    
+    Variable v : E.e tags_t.
+    
+    Hypothesis Hv : value v.
+    
+    Lemma canonical_forms_bool :
+      ⟦ errs, Γ ⟧ ⊢ v ∈ Bool -> exists b i, v = <{ BOOL b @ i }>.
+    Proof. crush_canonical. Qed.
+    
+    Lemma canonical_forms_bit : forall w,
+        ⟦ errs, Γ ⟧ ⊢ v ∈ bit<w> -> exists n i, v = <{ w W n @ i }>.
+    Proof. crush_canonical. Qed.
+    
+    Lemma canonical_forms_int : forall w,
+        ⟦ errs, Γ ⟧ ⊢ v ∈ int<w> -> exists z i, v = <{ w S z @ i }>.
+    Proof. crush_canonical. Qed.
+    
+    Lemma canonical_forms_tuple : forall ts,
+        ⟦ errs, Γ ⟧ ⊢ v ∈ tuple ts -> exists es i, v = <{ tup es @ i }>.
+    Proof. crush_canonical. Qed.
+    
+    Lemma canonical_forms_struct : forall ts,
+        ⟦ errs, Γ ⟧ ⊢ v ∈ struct { ts } -> exists fs i, v = <{ struct { fs } @ i }>.
+    Proof. crush_canonical. Qed.
+    
+    Lemma canonical_forms_header : forall ts,
+        ⟦ errs, Γ ⟧ ⊢ v ∈ hdr { ts } -> exists fs b i, v = <{ hdr { fs } valid:=b @ i }>.
+    Proof. crush_canonical. Qed.
+    
+    Lemma canonical_forms_error :
+      ⟦ errs, Γ ⟧ ⊢ v ∈ error -> exists err i, v = <{ Error err @ i }>.
+    Proof. crush_canonical. Qed.
+    
+    Lemma canonical_forms_matchkind :
+      ⟦ errs, Γ ⟧ ⊢ v ∈ matchkind -> exists mk i, v = <{ Matchkind mk @ i }>.
+    Proof. crush_canonical. Qed.
+    
+    Lemma canonical_forms_headerstack : forall ts n,
+        ⟦ errs, Γ ⟧ ⊢ v ∈ stack ts[n] ->
+        exists hs ni i, v = <{ Stack hs:ts[n] nextIndex:= ni @ i }>.
+    Proof. crush_canonical. Qed.
+  End CanonicalForms.
+  
+  Ltac inv_eq_val_expr :=
+    match goal with
+    | H: <{ BOOL _ @ _ }> = <{ BOOL _ @ _ }> |- _ => inv H
+    | H: <{ _ W _ @ _ }> = <{ _ W _ @ _ }> |- _ => inv H
+    | H: <{ _ S _ @ _ }> = <{ _ S _ @ _ }> |- _ => inv H
+    | H: <{ tup _ @ _ }> = <{ tup _ @ _ }> |- _ => inv H
+    | H: <{ struct { _ } @ _ }> = <{ struct { _ } @ _ }> |- _ => inv H
+    | H: <{ hdr { _ } valid:=_ @ _ }> = <{ hdr { _ } valid:=_ @ _ }>
+      |- _ => inv H
+    | H: <{ Stack _:_[_] nextIndex:=_ @ _ }> = <{ Stack _:_[_] nextIndex:=_ @ _ }>
+      |- _ => inv H
+    end.
+  (**[]*)
+  
+  Ltac assert_canonical_forms :=
+    match goal with
+    | Hv: value ?v, Ht: ⟦ _, _ ⟧ ⊢ ?v ∈ Bool |- _
+      => pose proof canonical_forms_bool _ _ _ Hv Ht as [? [? Hcanon]];
+        inv Hcanon; inv Hv; inv Ht
+    | Hv: value ?v, Ht: ⟦ _, _ ⟧ ⊢ ?v ∈ bit<_> |- _
+      => pose proof canonical_forms_bit _ _ _ Hv _ Ht as [? [? Hcanon]];
+        inv Hcanon; inv Hv; inv Ht
+    | Hv: value ?v, Ht: ⟦ _, _ ⟧ ⊢ ?v ∈ int<_> |- _
+      => pose proof canonical_forms_int _ _ _ Hv _ Ht as [? [? Hcanon]];
+        inv Hcanon; inv Hv; inv Ht
+    | Hv: value ?v, Ht: ⟦ _, _ ⟧ ⊢ ?v ∈ tuple _ |- _
+      => pose proof canonical_forms_tuple _ _ _ Hv _ Ht as [? [? Hcanon]];
+        inv Hcanon; inv Hv; inv Ht
+    | Hv: value ?v, Ht: ⟦ _, _ ⟧ ⊢ ?v ∈ struct { _ } |- _
+      => pose proof canonical_forms_struct _ _ _ Hv _ Ht as [? [? Hcanon]];
+        inv Hcanon; inv Hv; inv Ht
+    | Hv: value ?v, Ht: ⟦ _, _ ⟧ ⊢ ?v ∈ hdr { _ } |- _
+      => pose proof canonical_forms_header _ _ _ Hv _ Ht as [? [? [? Hcanon]]];
+        inv Hcanon; inv Hv; inv Ht
+    | Hv: value ?v, Ht: ⟦ _, _ ⟧ ⊢ ?v ∈ error |- _
+      => pose proof canonical_forms_error _ _ _ Hv Ht as [? [? Hcanon]];
+        inv Hcanon; inv Hv; inv Ht
+    | Hv: value ?v, Ht: ⟦ _, _ ⟧ ⊢ ?v ∈ matchkind |- _
+      => pose proof canonical_forms_matchkind _ _ _ Hv Ht as [? [? Hcanon]];
+        inv Hcanon; inv Hv; inv Ht
+    | Hv: value ?v, Ht: ⟦ _, _ ⟧ ⊢ ?v ∈ stack _[_] |- _
+      => pose proof canonical_forms_headerstack
+             _ _ _ Hv _ _ Ht as [? [? [? Hcanon]]];
+        inv Hcanon; inv Hv; inv Ht
+    end.
+  (**[]*)
+End CanonicalForms.
